Launchbury/AbstractTransform.thy
@@ -214,4 +214,5 @@ begin
   qed
 end
 
+
 end
