Launchbury/SestoftGC.thy
@@ -13,6 +13,7 @@ lemmas gc_step_intros[intro] =
 
 
 abbreviation gc_steps (infix "\<Rightarrow>\<^sub>G\<^sup>*" 50) where "gc_steps \<equiv> gc_step\<^sup>*\<^sup>*"
+lemmas converse_rtranclp_into_rtranclp[of gc_step, OF _ r_into_rtranclp, trans]
 
 lemma var_onceI:
   assumes "map_of \<Gamma> x = Some e"
@@ -25,6 +26,24 @@ proof-
   ultimately
   show ?thesis by (rule converse_rtranclp_into_rtranclp[OF _ r_into_rtranclp])
 qed
+
+lemma lam_and_restrict:
+  assumes "atom ` domA \<Delta> \<sharp>* \<Gamma>" and "atom ` domA \<Delta> \<sharp>* S"
+  assumes "V \<subseteq> domA \<Delta>"
+  shows "(\<Gamma>, Let \<Delta> e, S) \<Rightarrow>\<^sub>G\<^sup>* (restrictA V \<Delta> @ \<Gamma>, e, S)"
+proof-
+  from assms(1,2) have "(\<Gamma>, Let \<Delta> e, S) \<Rightarrow>\<^sub>G (\<Delta> @ \<Gamma>, e, S)"..
+  also
+  have "\<dots> \<Rightarrow>\<^sub>G (restrictA (V \<union> domA \<Gamma>) (\<Delta> @ \<Gamma>), e, S)"..
+  also
+  from fresh_distinct[OF assms(1)]
+  have "restrictA (V \<union> domA \<Gamma>) \<Delta> = restrictA V \<Delta>" by (induction \<Delta>) auto
+  hence "restrictA (V \<union> domA \<Gamma>) (\<Delta> @ \<Gamma>) = restrictA V \<Delta> @ \<Gamma>"
+    by (simp add: restrictA_append restrictA_noop)
+  finally show ?thesis.
+qed
+    
+  
 
 lemma normal_trans:  "c \<Rightarrow>\<^sup>* c' \<Longrightarrow> c \<Rightarrow>\<^sub>G\<^sup>* c'"
   by (induction rule:rtranclp_induct) (auto dest: normal)
